RegExp/Equiv.lean
@@ -1,0 +1,63 @@
+import RegExp.Basic
+
+namespace RegExp
+variable {α}
+
+def size (r : RegExp α) : Nat :=
+  suffices Nat from this.succ
+  match r with
+  | .nothing | ε | .single _ => 0
+  | .star r => r.size
+  | .append r₁ r₂ | .union r₁ r₂ => r₁.size + r₂.size
+
+example : @size α .nothing = 1 := rfl
+example : @size α ε = 1 := rfl
+example (a : α) : size (.single a) = 1 := rfl
+example {n} (r : RegExp α) : r.size = n → size r* = n + 1
+  | rfl => rfl
+example {n₁ n₂} (r₁ r₂ : RegExp α) : r₁.size = n₁ → r₂.size = n₂ → size (r₁ ++ r₂) = n₁ + n₂ + 1
+  | rfl, rfl => rfl
+example {n₁ n₂} (r₁ r₂ : RegExp α) : r₁.size = n₁ → r₂.size = n₂ → size (r₁ ∪ r₂) = n₁ + n₂ + 1
+  | rfl, rfl => rfl
+
+abbrev L (r : RegExp α) := {s : List α // s =~ r}
+
+instance setoid : Setoid (RegExp α) where
+  r r₁ r₂ := ∀ s, s =~ r₁ ↔ s =~ r₂
+  iseqv.refl _ _ := .rfl
+  iseqv.symm h s := (h s).symm
+  iseqv.trans h₁ h₂ s := (h₁ s).trans (h₂ s)
+
+variable {s : List α}
+
+theorem accept_nothing : ¬s =~ ∅ := nofun
+instance : Subsingleton (@L α ∅) where
+  allEq | _, ⟨_, h⟩ => absurd h accept_nothing
+
+instance : Inhabited (@L α ε) where
+  default := ⟨[], empty⟩
+instance : Subsingleton (@L α ε) where
+  allEq | ⟨_, empty⟩, ⟨_, empty⟩ => rfl
+theorem accept_empty : s =~ ε ↔ [] = s := ⟨fun | empty => rfl, fun | rfl => empty⟩
+
+variable {a b : α}
+
+instance : Inhabited (L (.single a)) where
+  default := ⟨[a], single⟩
+instance : Subsingleton (L (.single a)) where
+  allEq | ⟨_, single⟩, ⟨_, single⟩ => rfl
+theorem accept_single : s =~ a ↔ [a] = s := ⟨fun | single => rfl, fun | rfl => single⟩
+theorem accept_single_unique : [a] =~ b ↔ a = b :=
+  ⟨fun h => match accept_single.mp h with | rfl => rfl, fun | rfl => single⟩
+theorem accept_single_head (h : a::s =~ b) : a = b := match accept_single.mp h with | rfl => rfl
+theorem accept_single_tail (h : a::s =~ b) : [] = s := match accept_single.mp h with | rfl => rfl
+
+theorem accept_starEmpty : s =~ ∅* ↔ [] = s := ⟨fun | starEmpty => rfl, fun | rfl => starEmpty⟩
+example : (∅* : RegExp α) ≈ ε
+  | _ => ⟨fun | starEmpty => empty, fun | empty => starEmpty⟩
+
+variable {r : RegExp α}
+
+theorem accept_star (h : s =~ r) : s =~ r* := s.append_nil ▸ h.starAppend starEmpty
+example : r** ≈ r*
+  | s => ⟨_, accept_star⟩
